Prove existence of sound tick function

doc/coq/ALinking.v
@@ -1,7 +1,7 @@
 From MODULAR Require Export Abstract.
 Require Export Coq.Logic.FunctionalExtensionality.
 
-Generalizable Variables T.
+Generalizable Variables T BT AT.
 
 Definition inject_ctx_mem `{Eq T} (Cout : @dy_ctx T) (mem : T -> list expr_value) :=
   fun t => map (inject_ctx_v Cout) (mem t).
@@ -22,74 +22,264 @@ Proof.
   rewrite IHl. reflexivity.
 Qed.
 
-Definition delete_update `{time T} (Cout : @dy_ctx T) :=
+Inductive link {BT AT} :=
+  | BF (t : BT)
+  | AF (t : AT)
+.
+
+Definition link_eqb `{Eq BT} `{Eq AT} (t t' : @link BT AT) :=
+  match t, t' with
+  | BF t, BF t' => eqb t t'
+  | AF t, AF t' => eqb t t'
+  | _, _ => false
+  end.
+
+Lemma link_eqb_eq `{Eq BT} `{Eq AT} :
+  forall (t t' : @link BT AT), link_eqb t t' = true <-> t = t'.
+Proof.
+  intros.
+  destruct t; destruct t'; simpl; split; intros EQ; 
+  try rewrite eqb_eq in *;
+  try inversion EQ;
+  subst; eauto.
+Qed.
+
+Lemma link_eqb_neq `{Eq BT} `{Eq AT} :
+  forall (t t' : @link BT AT), link_eqb t t' = false <-> t <> t'.
+Proof.
+  intros. split; intros NEQ.
+  - red. intros contra. rewrite <- link_eqb_eq in contra.
+    rewrite NEQ in contra. inversion contra.
+  - refl_bool. intros contra. rewrite link_eqb_eq in contra.
+    apply NEQ. eauto.
+Qed.
+
+#[export] Instance link_eq `{Eq BT} `{Eq AT} : Eq (@link BT AT) :=
+  {
+    eqb := link_eqb;
+    eqb_eq := link_eqb_eq;
+    eqb_neq := link_eqb_neq
+  }.
+
+Fixpoint filter_ctx_bf {BT AT} (C : @dy_ctx (@link BT AT)) :=
+  match C with
+  | [||] => [||]
+  | dy_c_lam x t C' =>
+    match t with
+    | BF t => dy_c_lam x t (filter_ctx_bf C')
+    | AF t => filter_ctx_bf C'
+    end
+  | dy_c_lete x t C' =>
+    match t with
+    | BF t => dy_c_lete x t (filter_ctx_bf C')
+    | AF t => filter_ctx_bf C'
+    end
+  | dy_c_letm M C' C'' => dy_c_letm M (filter_ctx_bf C') (filter_ctx_bf C'')
+  end.
+
+Fixpoint filter_ctx_af {BT AT} (C : @dy_ctx (@link BT AT)) :=
+  match C with
+  | [||] => [||]
+  | dy_c_lam x t C' =>
+    match t with
+    | AF t => dy_c_lam x t (filter_ctx_af C')
+    | BF t => filter_ctx_af C'
+    end
+  | dy_c_lete x t C' =>
+    match t with
+    | AF t => dy_c_lete x t (filter_ctx_af C')
+    | BF t => filter_ctx_af C'
+    end
+  | dy_c_letm M C' C'' => dy_c_letm M (filter_ctx_af C') (filter_ctx_af C'')
+  end.
+
+Definition filter_v_bf {BT AT} (v : @expr_value (@link BT AT)) :=
+  match v with
+  | Closure x e C => Closure x e (filter_ctx_bf C)
+  end.
+
+Definition filter_v_af {BT AT} (v : @expr_value (@link BT AT)) :=
+  match v with
+  | Closure x e C => Closure x e (filter_ctx_af C)
+  end.
+
+Definition filter_mem_bf {BT AT} (mem : (@link BT AT) -> list (@expr_value (@link BT AT))) :=
+  fun t => map filter_v_bf (mem (BF t))
+.
+
+Definition filter_mem_af {BT AT} (mem : (@link BT AT) -> list (@expr_value (@link BT AT))) :=
+  fun t => map filter_v_af (mem (AF t))
+.
+
+Fixpoint lift_ctx_bf {BT AT} C : @dy_ctx (@link BT AT) :=
+  match C with
+  | [||] => [||]
+  | dy_c_lam x t C' => dy_c_lam x (BF t) (lift_ctx_bf C')
+  | dy_c_lete x t C' => dy_c_lete x (BF t) (lift_ctx_bf C')
+  | dy_c_letm M C' C'' => dy_c_letm M (lift_ctx_bf C') (lift_ctx_bf C'')
+  end.
+
+Definition lift_v_bf {BT AT} v : @expr_value (@link BT AT) :=
+  match v with
+  | Closure x e C => Closure x e (lift_ctx_bf C)
+  end.
+
+Fixpoint lift_ctx_af {BT AT} C : @dy_ctx (@link BT AT) :=
+  match C with
+  | [||] => [||]
+  | dy_c_lam x t C' => dy_c_lam x (AF t) (lift_ctx_af C')
+  | dy_c_lete x t C' => dy_c_lete x (AF t) (lift_ctx_af C')
+  | dy_c_letm M C' C'' => dy_c_letm M (lift_ctx_af C') (lift_ctx_af C'')
+  end.
+
+Definition lift_v_af {BT AT} v : @expr_value (@link BT AT) :=
+  match v with
+  | Closure x e C => Closure x e (lift_ctx_af C)
+  end.
+
+Definition link_tick `{time BT} `{time AT} (Cout : @dy_ctx BT) :=
   fun C st x v =>
     match st with
     | ST mem t =>
-      update (delete_inject Cout C)
-             (ST (delete_ctx_mem Cout mem) t)
-             x (delete_ctx_v Cout v)
+      match t with
+      | BF t => BF (tick (filter_ctx_bf C) (ST (filter_mem_bf mem) t) x (filter_v_bf v))
+      | AF t =>
+        let Cout := lift_ctx_bf Cout in
+        AF
+        (tick (filter_ctx_af (delete_ctx Cout C))
+                (ST (filter_mem_af (delete_ctx_mem Cout mem)) t)
+                x (filter_v_af (delete_ctx_v Cout v)))
+      end
     end.
 
-#[export] Instance delete_time `{time T} (Cout : @dy_ctx T) : time :=
+#[export] Instance link_time `{time BT} `{time AT} (Cout : @dy_ctx BT) : (@time (@link BT AT) (@link_eq BT _ AT _)) :=
   {
-    update := delete_update Cout
+    tick := link_tick Cout
   }.
 
-Lemma delete_update_eq `{time T} (Cout : @dy_ctx T) :
-  forall C mem t x v,
-    delete_update Cout (Cout<|C|>) (ST (inject_ctx_mem Cout mem) t) x (inject_ctx_v Cout v) =
-    update C (ST mem t) x v.
+Definition link_mem `{Eq BT} `{Eq AT}
+  (bmem : BT -> list (@expr_value BT)) (Cout : @dy_ctx BT)
+  (amem : AT -> list (@expr_value AT)) : (@link BT AT) -> list (@expr_value (@link BT AT)):=
+  fun t =>
+    match t with
+    | BF t => map lift_v_bf (bmem t)
+    | AF t => map (inject_ctx_v (lift_ctx_bf Cout)) (map (lift_v_af) (amem t))
+    end.
+
+Lemma filter_lift_eq_af {BT AT} :
+  forall (C : @dy_ctx AT),
+    filter_ctx_af (@lift_ctx_af BT AT C) = C.
 Proof.
-  intros. destruct v. unfold inject_ctx_v.
-  unfold delete_update. simpl.
-  rewrite delete_inject_eq. rewrite delete_ctx_mem_eq.
-  rewrite delete_inject_eq. reflexivity.
+  induction C; simpl; try rewrite IHC; eauto.
+  rewrite IHC2. rewrite IHC1. eauto.
 Qed.
 
-Lemma plugin_map_assoc :
-  forall `{Eq T} (Cout C C' : @dy_ctx T),
-    (map_inject Cout C) [|map_inject Cout C'|] = (map_inject Cout (C [|C'|])).
+Lemma filter_lift_eq_bf {BT AT} :
+  forall (C : @dy_ctx BT),
+    filter_ctx_bf (@lift_ctx_bf BT AT C) = C.
 Proof.
-  intros. revert Cout C'. induction C; intros; simpl; eauto; try rewrite IHC; try rewrite IHC2; eauto.
+  induction C; simpl; try rewrite IHC; eauto.
+  rewrite IHC2. rewrite IHC1. eauto.
 Qed.
 
-Lemma plugin_inject_assoc :
-  forall `{Eq T} (Cout C C' : @dy_ctx T),
-    (Cout <| C |>)[| map_inject Cout C' |] = (Cout <|C[|C'|]|>).
-Proof.
-  intros. unfold inject_ctx. rewrite <- c_plugin_assoc.
-  rewrite plugin_map_assoc. eauto.
-Qed.
-
-Lemma inject_update_m_eq :
-  forall `{Eq T} t x e mem (Cout C : @dy_ctx T),
-  (t !#-> Closure x e (Cout <| C |>); inject_ctx_mem Cout mem) =
-            inject_ctx_mem Cout (t !#-> Closure x e C; mem).
+Lemma filter_delete_eq `{time BT} `{time AT} (Cout : @dy_ctx BT):
+  forall bmem amem,
+  filter_mem_af
+    (delete_ctx_mem (lift_ctx_bf Cout)
+    (link_mem bmem Cout amem)) = amem.
 Proof.
   intros. apply functional_extensionality.
-  intros. unfold update_m. unfold inject_ctx_mem.
-  destruct (eqb x0 t); eauto.
+  intros. unfold filter_mem_af.
+  unfold delete_ctx_mem. simpl.
+  remember (lift_ctx_bf Cout) as vout eqn:E. clear E.
+  remember (amem x) as l eqn:E. clear E.
+  induction l; simpl; eauto.
+  rewrite IHl. destruct a. simpl.
+  rewrite delete_inject_eq. rewrite filter_lift_eq_af. eauto.
 Qed.
 
-Lemma delete_eval_eq {T} `{ET : Eq T} `{TT : @time T ET} (Cout : @dy_ctx T) :
-  forall C st e v st'
-         (EVAL : @EvalR T ET TT C st e v st'),
+Lemma link_tick_eq `{time BT} `{time AT} (Cout : @dy_ctx BT) :
+  forall bmem C amem t x v,
+    link_tick Cout ((lift_ctx_bf Cout)<|(lift_ctx_af C)|>)
+                (ST (link_mem bmem Cout amem) (AF t)) x 
+                (inject_ctx_v (lift_ctx_bf Cout) (lift_v_af v)) =
+    AF (tick C (ST amem t) x v).
+Proof.
+  intros. destruct v. unfold inject_ctx_v. simpl.
+  rewrite delete_inject_eq.
+  rewrite delete_inject_eq.
+  rewrite filter_delete_eq.
+  rewrite filter_lift_eq_af. rewrite filter_lift_eq_af.
+  reflexivity.
+Qed.
+
+Lemma link_update_m_eq `{time BT} `{time AT} (Cout : @dy_ctx BT):
+  forall bmem amem t v,
+  (AF t !#-> inject_ctx_v (lift_ctx_bf Cout) (lift_v_af v);
+    (link_mem bmem Cout amem)) =
+    link_mem bmem Cout (t !#-> v; amem).
+Proof.
+  intros. apply functional_extensionality.
+  intros. unfold update_m. destruct v. simpl.
+  destruct x; simpl; eauto.
+  destruct (eqb t0 t); eauto.
+Qed.
+
+Lemma lift_addr_x {BT AT} :
+  forall (C : @dy_ctx AT) x,
+    addr_x (lift_ctx_af C : @dy_ctx (@link BT AT)) x =
+      match addr_x C x with
+      | Some addr => Some (AF addr)
+      | None => None
+      end.
+Proof.
+  induction C; simpl; eauto;
+  intros;
+  destruct (eq_eid x0 x); rewrite IHC;
+  destruct (addr_x C x0); eauto.
+Qed.
+
+Lemma lift_ctx_M {BT AT} :
+  forall (C : @dy_ctx AT) M,
+    ctx_M (lift_ctx_af C : @dy_ctx (@link BT AT)) M =
+      match ctx_M C M with
+      | Some CM => Some (lift_ctx_af CM)
+      | None => None
+      end.
+Proof.
+  induction C; simpl; eauto;
+  intros.
+  destruct (eq_mid M0 M); rewrite IHC2;
+  destruct (ctx_M C2 M0); eauto.
+Qed.
+
+Lemma lift_plugin_af {BT AT} :
+  forall (C C' : @dy_ctx AT),
+    @lift_ctx_af BT AT (C[|C'|]) = (lift_ctx_af C [|lift_ctx_af C'|]).
+Proof.
+  induction C; simpl; intros; try rewrite IHC; eauto.
+  rewrite IHC2. eauto.
+Qed.
+
+Lemma delete_eval_eq `{time BT} `{time AT} (Cout : @dy_ctx BT) :
+  forall bmem C st e v st'
+         (EVAL : @EvalR AT _ _ C st e v st'),
+    let inject_C := (lift_ctx_bf Cout) <|(lift_ctx_af C)|> in
     let inject_v :=
       match v with
-      | EVal (Closure x_v e_v C_v) => EVal (Closure x_v e_v (Cout<|C_v|>))
-      | MVal C_v => MVal (Cout<|C_v|>)
+      | EVal ev => EVal (inject_ctx_v (lift_ctx_bf Cout) (lift_v_af ev))
+      | MVal C_v => MVal ((lift_ctx_bf Cout)<|(lift_ctx_af C_v)|>)
       end in
     let inject_st :=
       match st with
-      | ST mem t => ST (inject_ctx_mem Cout mem) t
+      | ST amem t => ST (link_mem bmem Cout amem) (AF t)
       end in
     let inject_st' :=
       match st' with
-      | ST mem' t' => ST (inject_ctx_mem Cout mem') t'
+      | ST amem' t' => ST (link_mem bmem Cout amem') (AF t')
       end in
-    @EvalR T ET (@delete_time T ET TT Cout)
-      (Cout<|C|>) inject_st e inject_v inject_st'.
+    @EvalR (@link BT AT) _ (link_time Cout)
+      inject_C inject_st e inject_v inject_st'.
 Proof.
   intros. induction EVAL;
   try destruct v; try destruct st; try destruct st'; try destruct st'';
@@ -98,34 +288,42 @@ Proof.
   try (destruct inject_st' eqn:INJst'; inversion INJst'; subst); eauto.
   - inversion STATE; subst.
     eapply Eval_var_e; eauto.
-    pose proof (inject_ctx_addr_x x Cout C) as RR.
+    pose proof (inject_ctx_addr_x x (lift_ctx_bf Cout) (lift_ctx_af C)) as RR.
+    rewrite lift_addr_x in RR.
     rewrite <- ADDR in RR. symmetry. apply RR.
-    unfold inject_ctx_mem. 
+    unfold link_mem. 
     remember (mem0 addr) as l.
-    clear Heql C mem0 x addr t0 inject_st' INJst' STATE inject_st INJst ADDR inject_v INJv.
+    clear Heql inject_C C mem0 x addr t0 inject_st' INJst' STATE inject_st INJst ADDR inject_v INJv.
     revert Cout x0 e C0 ACCESS. induction l; simpl; intros; eauto.
     destruct ACCESS as [L | R].
     left. rewrite L. simpl. eauto.
     right. apply IHl. eauto.
   - destruct st_v. destruct arg.
     eapply Eval_app. apply IHEVAL1. apply IHEVAL2.
-    pose proof (delete_update_eq Cout C mem t x (Closure x1 e3 C1)) as RR.
-    simpl in *. rewrite RR. clear RR.
-    rewrite inject_update_m_eq.
-    replace (dy_c_lam x t ([||])) with (map_inject Cout (dy_c_lam x t ([||]))) by reflexivity.
-    rewrite plugin_inject_assoc. eauto.
-  - pose proof (inject_ctx_ctx_M M Cout C) as RR. 
+    pose proof (link_tick_eq Cout bmem C mem t x (Closure x1 e3 C1)) as RR.
+    simpl in *. replace inject_C with (lift_ctx_bf Cout <| lift_ctx_af C |>) by reflexivity.
+    rewrite RR. clear RR.
+    pose proof (link_update_m_eq Cout bmem mem t (Closure x1 e3 C1)) as RR. simpl in RR.
+    rewrite RR. clear RR.
+    replace (dy_c_lam x (AF t) ([||])) with (map_inject (lift_ctx_bf Cout) (dy_c_lam x (AF t) ([||]))) by reflexivity.
+    rewrite plugin_inject_assoc. rewrite lift_plugin_af in IHEVAL3. eauto.
+  - pose proof (inject_ctx_ctx_M M (lift_ctx_bf Cout) (lift_ctx_af C)) as RR.
+    rewrite lift_ctx_M in RR.
     rewrite <- ACCESS in RR.
     eapply Eval_var_m; eauto.
   - eapply Eval_lete; eauto.
-    pose proof (delete_update_eq Cout C mem t x (Closure x0 e0 C0)) as RR.
-    simpl in *. rewrite RR. clear RR.
-    rewrite inject_update_m_eq.
-    replace (dy_c_lete x t ([||])) with (map_inject Cout (dy_c_lete x t ([||]))) by reflexivity.
-    rewrite plugin_inject_assoc. eauto.
+    pose proof (link_tick_eq Cout bmem C mem t x (Closure x0 e0 C0)) as RR.
+    simpl in *. replace inject_C with (lift_ctx_bf Cout <| lift_ctx_af C |>) by reflexivity.
+    rewrite RR. clear RR.
+    pose proof (link_update_m_eq Cout bmem mem t (Closure x0 e0 C0)) as RR. simpl in RR.
+    rewrite RR. clear RR.
+    replace (dy_c_lete x (AF t) ([||])) with (map_inject (lift_ctx_bf Cout) (dy_c_lete x (AF t) ([||]))) by reflexivity.
+    rewrite plugin_inject_assoc. rewrite lift_plugin_af in IHEVAL2. eauto.
   - eapply Eval_letm; eauto.
-    assert ((Cout <| C |>) [|dy_c_letm M (Cout <| C' |>) ([||])|] =
-            (Cout <| (C [|dy_c_letm M C' ([||])|]) |>)) as RR. 
-    { rewrite <- plugin_inject_assoc. simpl. eauto. } 
+    assert (inject_C [|dy_c_letm M (lift_ctx_bf Cout <| lift_ctx_af C' |>) ([||])|] =
+            (lift_ctx_bf Cout <| lift_ctx_af (C [|dy_c_letm M C' ([||])|]) |>)) as RR. 
+    { replace inject_C with (lift_ctx_bf Cout <| lift_ctx_af C |>) by reflexivity.
+      rewrite lift_plugin_af.
+      rewrite <- plugin_inject_assoc. simpl. eauto. } 
     rewrite RR. clear RR. simpl in *. exact IHEVAL2.
 Qed.
